> è¯•è¯æ˜ï¼Œå¯¹äºå‚æ•° $\boldsymbol w$ï¼Œé€»è¾‘æ–¯è°›å›å½’çš„ç›®æ ‡å‡½æ•° $(3.18)$ æ˜¯éğŸœ·çš„ï¼Œä½†å…¶å¯¹æ•°ä¼¼ç„¶å‡½æ•° $(3.27)$ æ˜¯ğŸœ·çš„ã€‚

å¯¹äº $(3.18)$ï¼š

$$
f(\boldsymbol w)=\dfrac1{1+\mathrm e^{-(\boldsymbol w^\mathrm T\boldsymbol x+b)}}
$$

$$
\mathbf{grad} f(\boldsymbol w)=\dfrac{\boldsymbol x^\mathrm T\mathrm e^{-(\boldsymbol w^\mathrm T\boldsymbol x+b)}}{(1+\mathrm e^{-(\boldsymbol w^\mathrm T\boldsymbol x+b)})^2}=\boldsymbol x(f(\boldsymbol w)-f^2(\boldsymbol w))
$$

$$
\mathbf{grad}^2f(\boldsymbol w)=\boldsymbol x(1-2f(\boldsymbol w))\mathbf{grad}^\mathrm T f(\boldsymbol w)=\boldsymbol x\boldsymbol x^\mathrm T(1-2f(\boldsymbol w))(f(\boldsymbol w)-f^2(\boldsymbol w))
$$

è€ƒè™‘ä»»æ„éé›¶å‘é‡ $\boldsymbol y\in \mathbb R^d$ï¼Œæœ‰

$$
\boldsymbol y^\mathrm T\boldsymbol x\boldsymbol x^\mathrm T\boldsymbol y=(\boldsymbol y^\mathrm T{\boldsymbol x}_i)^2\ge0
$$

æ•… $\boldsymbol x\boldsymbol x^\mathrm T$ åŠæ­£å®šï¼Œè€Œ $f(\boldsymbol w)\in(0.5,1)$ æ—¶æœ‰ $(1-2f(\boldsymbol w))(f(\boldsymbol w)-f^2(\boldsymbol w))<0$ï¼Œæ•… $f(\boldsymbol w)$ ä¸æ˜¯ğŸœ·çš„ã€‚

----

å¯¹äº $(3.27)$ï¼š

$$
\ln L({\boldsymbol w})=\sum_{i=1}^m\left(y_i{\boldsymbol w}^\mathrm T{\boldsymbol x}_i-\ln(1+\mathrm e^{{\boldsymbol w}^\mathrm T{\boldsymbol x}_i})\right)
$$

$$\mathbf{grad} (-\ln L({\boldsymbol w}))=-\sum_{i=1}^m{\boldsymbol x}_i\left({y_i}-\dfrac{\mathrm e^{{\boldsymbol w}^\mathrm T{\boldsymbol x}_i}}{1+\mathrm e^{{\boldsymbol w}^\mathrm T{\boldsymbol x}_i}}\right)=-\sum _{i=1}^m{\boldsymbol x}_i\left({y_i}-\pi({\boldsymbol x}_i)\right)$$

$$
\mathbf{grad}^2(-\ln L({\boldsymbol w}))=\sum_{i=1}^m{\boldsymbol x}_i\cdot\dfrac{{\boldsymbol x}_i^\mathrm T\mathrm e^{{\boldsymbol w}^\mathrm T{\boldsymbol x}_i}}{\left(1+\mathrm e^{{\boldsymbol w}^\mathrm T{\boldsymbol x}_i}\right)^2}=\sum _{i=1}^m{\boldsymbol x}_i{\boldsymbol x}_i^\mathrm T\cdot\pi({\boldsymbol x}_i)\cdot(1-\pi({\boldsymbol x}_i))
$$

å…¶ä¸­ $\boldsymbol x_i\boldsymbol x_i^\mathrm T$ åŠæ­£å®šï¼Œè€Œ $\pi({\boldsymbol x}_i)\cdot(1-\pi({\boldsymbol x}_i))\ge0$ï¼Œæ•… $\mathbf{grad}^2(-\ln L({\boldsymbol w}))$ åŠæ­£å®šï¼Œå³ $-\ln L({\boldsymbol w})$ æ˜¯ğŸœ·çš„ã€‚
