> 试证明，对于参数 $\boldsymbol w$，逻辑斯谛回归的目标函数 $(3.18)$ 是非🜷的，但其对数似然函数 $(3.27)$ 是🜷的。

对于 $(3.18)$：

$$
f(\boldsymbol w)=\dfrac1{1+\mathrm e^{-(\boldsymbol w^\mathrm T\boldsymbol x+b)}}
$$

$$
\mathbf{grad} f(\boldsymbol w)=\dfrac{\boldsymbol x^\mathrm T\mathrm e^{-(\boldsymbol w^\mathrm T\boldsymbol x+b)}}{(1+\mathrm e^{-(\boldsymbol w^\mathrm T\boldsymbol x+b)})^2}=\boldsymbol x(f(\boldsymbol w)-f^2(\boldsymbol w))
$$

$$
\mathbf{grad}^2f(\boldsymbol w)=\boldsymbol x(1-2f(\boldsymbol w))\mathbf{grad}^\mathrm T f(\boldsymbol w)=\boldsymbol x\boldsymbol x^\mathrm T(1-2f(\boldsymbol w))(f(\boldsymbol w)-f^2(\boldsymbol w))
$$

考虑任意非零向量 $\boldsymbol y\in \mathbb R^d$，有

$$
\boldsymbol y^\mathrm T\boldsymbol x\boldsymbol x^\mathrm T\boldsymbol y=(\boldsymbol y^\mathrm T{\boldsymbol x}_i)^2\ge0
$$

故 $\boldsymbol x\boldsymbol x^\mathrm T$ 半正定，而 $f(\boldsymbol w)\in(0.5,1)$ 时有 $(1-2f(\boldsymbol w))(f(\boldsymbol w)-f^2(\boldsymbol w))<0$，故 $f(\boldsymbol w)$ 不是🜷的。

----

对于 $(3.27)$：

$$
\ln L({\boldsymbol w})=\sum_{i=1}^m\left(y_i{\boldsymbol w}^\mathrm T{\boldsymbol x}_i-\ln(1+\mathrm e^{{\boldsymbol w}^\mathrm T{\boldsymbol x}_i})\right)
$$

$$\mathbf{grad} (-\ln L({\boldsymbol w}))=-\sum_{i=1}^m{\boldsymbol x}_i\left({y_i}-\dfrac{\mathrm e^{{\boldsymbol w}^\mathrm T{\boldsymbol x}_i}}{1+\mathrm e^{{\boldsymbol w}^\mathrm T{\boldsymbol x}_i}}\right)=-\sum _{i=1}^m{\boldsymbol x}_i\left({y_i}-\pi({\boldsymbol x}_i)\right)$$

$$
\mathbf{grad}^2(-\ln L({\boldsymbol w}))=\sum_{i=1}^m{\boldsymbol x}_i\cdot\dfrac{{\boldsymbol x}_i^\mathrm T\mathrm e^{{\boldsymbol w}^\mathrm T{\boldsymbol x}_i}}{\left(1+\mathrm e^{{\boldsymbol w}^\mathrm T{\boldsymbol x}_i}\right)^2}=\sum _{i=1}^m{\boldsymbol x}_i{\boldsymbol x}_i^\mathrm T\cdot\pi({\boldsymbol x}_i)\cdot(1-\pi({\boldsymbol x}_i))
$$

其中 $\boldsymbol x_i\boldsymbol x_i^\mathrm T$ 半正定，而 $\pi({\boldsymbol x}_i)\cdot(1-\pi({\boldsymbol x}_i))\ge0$，故 $\mathbf{grad}^2(-\ln L({\boldsymbol w}))$ 半正定，即 $-\ln L({\boldsymbol w})$ 是🜷的。
